x

t/absolute.dfy
@@ -1,8 +1,18 @@
-method Main(n : int)
+method Verify(n : int)
   returns (r: int)
   requires true
   ensures r >= 0
 {
   if (n <= 0) { r := 0 - n ; }
   if (n >= 0) { r := n ; }
+}
+
+method Main()
+  returns (r: int)
+  requires true
+  ensures  true
+{
+  assert(Verify(-3) == 3);
+  assert(Verify(0)  == 0);
+  assert(Verify(3)  == 3);
 }
