t/straight-line.dfy
@@ -1,8 +1,17 @@
-method Main(x: int)
+method Verify(x: int)
   returns (r: int)
   requires x > 0
   ensures r > 0
 {
   r := 2 * x ;
   r := r * x ;
+}
+
+method Main()
+  returns (r: int)
+  requires true
+  ensures  true
+{
+  assert(Verify(0) == 0);
+  assert(Verify(3) == 18);
 }
