t/sum-to-n.dfy
@@ -1,4 +1,4 @@
-method Main(n : int) returns (r : int)
+method Verify(n : int) returns (r : int)
   requires n >= 0
   ensures  r == n*(n + 1) / 2
 {
@@ -12,4 +12,13 @@ method Main(n : int) returns (r : int)
     r := r + i;
     i := i - 1;
   }
+}
+
+method Main()
+  returns (r: int)
+  requires true
+  ensures  true
+{
+  assert(Verify(0)  == 0);
+  assert(Verify(3) == 6);
 }
