t/double.dfy
@@ -4,3 +4,13 @@ method Main(n : int) returns (r : int)
 {
   r := n * 2 ;
 }
+
+method Main()
+  returns (r: int)
+  requires true
+  ensures  true
+{
+  assert(Verify(0) == 0);
+  assert(Verify(10) == 20);
+  assert(Verify(-10) == -20);
+}
